lib: Check in sorting routine

src/Utils/Library.dfy
@@ -1,5 +1,4 @@
-module Utils.Lib {
-module ControlFlow {
+module Utils.Lib.ControlFlow {
   function method Unreachable<A>() : A
     requires false
   {
@@ -7,7 +6,7 @@ module ControlFlow {
   }
 }
 
-module Debug {
+module Utils.Lib.Debug {
   class {:compile false} Debugger {
     static method {:extern "System.Diagnostics.Debugger", "Break"} Break() {}
   }
@@ -20,7 +19,7 @@ module Debug {
   }
 }
 
-module Datatypes {
+module Utils.Lib.Datatypes {
   datatype Option<+T> = | Some(value: T) | None
   {
     function method UnwrapOr(default: T) : T {
@@ -93,7 +92,7 @@ module Datatypes {
   }
 }
 
-module Seq {
+module Utils.Lib.Seq {
   // FIXME why not use a comprehension directly?
   function method {:opaque} Map<T, Q>(f: T ~> Q, ts: seq<T>) : (qs: seq<Q>)
     reads f.reads
@@ -276,7 +275,24 @@ module Seq {
   }
 }
 
-module Str {
+module Utils.Lib.Outcome.OfSeq { // FIXME rename to Seq
+  import Seq
+  import opened Datatypes
+
+  function method Combine<E>(so: seq<Outcome<E>>): (os: Outcome<seq<E>>)
+    ensures os.Pass? ==> forall o | o in so :: o.Pass?
+    ensures os.Pass? <== forall o | o in so :: o.Pass?
+  {
+    var fails := Seq.Filter(so, (x: Outcome<E>) => x.Fail?);
+    if |fails| == 0 then
+      Pass
+    else
+      assert fails[0] in so;
+      Fail(Seq.Map((x: Outcome<E>) requires x.Fail? => x.error, fails))
+  }
+}
+
+module Utils.Lib.Str {
 module Private {
   function method digits(n: int, base: int): (digits: seq<int>)
     requires base > 1
@@ -355,7 +371,203 @@ module Private {
   }
 }
 
-module Math {
+module Utils.Lib.Set {
+  function method Map<T, T'>(ts: set<T>, f: T ~> T'): set<T'>
+    reads set t <- ts, o <- f.reads(t) :: o
+    requires forall t <- ts :: f.requires(t)
+  {
+    set t <- ts :: f(t)
+  }
+
+  function method OfSeq<T(==)>(sq: seq<T>): set<T> {
+    set x <- sq
+  }
+
+  function method OfSlice<T(==)>(arr: array<T>, lo: int, hi: int): set<T>
+    requires 0 <= lo <= hi <= arr.Length
+    reads arr
+  {
+    OfSeq(arr[lo..hi])
+  }
+
+  function method OfArray<T(==)>(arr: array<T>): set<T>
+    reads arr
+  {
+    OfSlice(arr, 0, arr.Length)
+  }
+}
+
+module Utils.Lib.Multiset {
+  function method OfSlice<T(==)>(arr: array<T>, lo: int, hi: int): multiset<T>
+    requires 0 <= lo <= hi <= arr.Length
+    reads arr
+  {
+    multiset(arr[lo..hi])
+  }
+
+  function method OfArray<T(==)>(arr: array<T>): multiset<T>
+    reads arr
+  {
+    OfSlice(arr, 0, arr.Length)
+  }
+}
+
+module Utils.Lib.Array {
+  import Set
+  import Multiset
+
+  method OfSet<T>(st: set<T>) returns (arr: array<T>)
+    ensures fresh(arr)
+    ensures Set.OfArray(arr) == st
+    ensures Multiset.OfArray(arr) == multiset(st)
+  {
+    if |st| == 0 {
+      arr := new T[|st|];
+    } else {
+      var s := st;
+      var t0 :| t0 in s;
+      arr := new T[|st|](_ => t0);
+      for i := 0 to |s|
+        invariant |s| == |st| - i
+        invariant Set.OfSlice(arr, 0, i) + s == st
+        invariant Multiset.OfSlice(arr, 0, i) + multiset(s) == multiset(st)
+      {
+        var t :| t in s;
+        arr[i] := t;
+        s := s - {t};
+        assert Set.OfSlice(arr, 0, i + 1) == Set.OfSlice(arr, 0, i) + {t};
+      }
+    }
+  }
+}
+
+module Utils.Lib.Int.Comparison {
+  import C = Sort.Comparison
+
+  function method Cmp(i0: int, i1: int): C.Cmp {
+    if i0 < i1 then C.Lt
+    else if i0 > i1 then C.Gt
+    else C.Eq
+  }
+
+  const Comparison := C.Comparison(Cmp);
+
+  lemma {:induction ints} Total(ints: set<int>)
+    ensures Comparison.Total?(ints)
+  {}
+}
+
+module Utils.Lib.Char.Comparison {
+  import C = Sort.Comparison
+
+  function method Cmp(i0: char, i1: char): C.Cmp {
+    if i0 < i1 then C.Lt
+    else if i0 > i1 then C.Gt
+    else C.Eq
+  }
+
+  const Comparison := C.Comparison(Cmp);
+
+  lemma {:induction chars} Total(chars: set<char>)
+    ensures Comparison.Total?(chars)
+  {}
+}
+
+module Utils.Lib.Seq.Comparison {
+  import Set
+  import C = Sort.Comparison
+
+  function Flatten<T>(tss: set<seq<T>>): set<T> {
+    set ts <- tss, t <- ts :: t
+  }
+
+  datatype SeqComparison<!T> = SeqComparison(cmp: C.Comparison<T>) {
+    function method Cmp(s0: seq<T>, s1: seq<T>): C.Cmp {
+      if s0 == [] && s1 == [] then C.Eq
+      else if s0 == [] then C.Lt
+      else if s1 == [] then C.Gt
+      else
+        match cmp.Compare(s0[0], s1[0])
+          case Eq => Cmp(s0[1..], s1[1..])
+          case other => other
+    }
+
+    const Comparison := C.Comparison(Cmp);
+
+    lemma {:induction false} Complete1(s0: seq<T>, s1: seq<T>)
+      requires cmp.Total?(Set.OfSeq(s0) + Set.OfSeq(s1))
+      ensures Comparison.Complete??(s0, s1)
+    {
+      if s0 != [] && s1 != [] {
+        assert s0[0] in s0 && s1[0] in s1;
+        assert s0[0] in Set.OfSeq(s0) && s1[0] in Set.OfSeq(s1);
+        Complete1(s0[1..], s1[1..]);
+      }
+    }
+
+    lemma {:induction false} Antisymmetric1(s0: seq<T>, s1: seq<T>)
+      requires cmp.Total?(Set.OfSeq(s0) + Set.OfSeq(s1))
+      ensures Comparison.Antisymmetric??(s0, s1)
+    {
+      // forall s0, s1 | s0 in tss && s1 in tss ensures Comparison.Complete??(s0, s1) {
+      if s0 != [] && s1 != [] {
+        assert s0[0] in s0 && s1[0] in s1;
+        assert s0[0] in Set.OfSeq(s0) && s1[0] in Set.OfSeq(s1);
+        assert s0 == [s0[0]] + s0[1..] && s1 == [s1[0]] + s1[1..];
+        Antisymmetric1(s0[1..], s1[1..]);
+      }
+    }
+
+    lemma {:induction false} Transitive1(s0: seq<T>, s1: seq<T>, s2: seq<T>)
+      requires cmp.Total?(Set.OfSeq(s0) + Set.OfSeq(s1) + Set.OfSeq(s2))
+      ensures Comparison.Transitive??(s0, s1, s2)
+    {
+      if s0 != [] && s1 != [] && s1 != [] && Comparison.Compare(s0, s1).Le? && Comparison.Compare(s1, s2).Le? {
+        assert s0[0] in s0 && s1[0] in s1 && s2[0] in s2;
+        assert s0[0] in Set.OfSeq(s0) && s1[0] in Set.OfSeq(s1) && s2[0] in Set.OfSeq(s2);
+        assert s0 == [s0[0]] + s0[1..] && s1 == [s1[0]] + s1[1..] && s2 == [s2[0]] + s2[1..];
+        assert cmp.Compare(s0[0], s1[0]).Le?;
+        assert cmp.Compare(s1[0], s2[0]).Le?;
+        assert cmp.Transitive??(s0[0], s1[0], s2[0]);
+        assert cmp.Compare(s0[0], s2[0]).Le?;
+        Transitive1(s0[1..], s1[1..], s2[1..]);
+      }
+    }
+
+    lemma {:induction false} Total(tss: set<seq<T>>)
+      requires cmp.Total?(Flatten(tss))
+      ensures Comparison.Total?(tss)
+    {
+      forall s0, s1 | s0 in tss && s1 in tss ensures Comparison.Complete??(s0, s1) {
+        Complete1(s0, s1);
+      }
+      forall s0, s1 | s0 in tss && s1 in tss ensures Comparison.Antisymmetric??(s0, s1) {
+        Antisymmetric1(s0, s1);
+      }
+      forall s0, s1, s2 | s0 in tss && s1 in tss && s2 in tss ensures Comparison.Transitive??(s0, s1, s2) {
+        Transitive1(s0, s1, s2);
+      }
+    }
+  }
+}
+
+module Utils.Lib.Str.Comparison {
+  import C = Sort.Comparison
+  import SeqCmp = Seq.Comparison
+  import CharCmp = Char.Comparison
+
+  const StrComparison := SeqCmp.SeqComparison(CharCmp.Comparison);
+  const Comparison := StrComparison.Comparison;
+
+  lemma {:induction false} Total(strs: set<string>)
+    ensures Comparison.Total?(strs)
+  {
+    CharCmp.Total(SeqCmp.Flatten(strs));
+    StrComparison.Total(strs);
+  }
+}
+
+module Utils.Lib.Math {
   function method {:opaque} Max(x: int, y: int) : (m: int)
     ensures x <= m
     ensures y <= m
@@ -369,4 +581,172 @@ module Math {
     else x * IntPow(x, n - 1)
   }
 }
+
+module Utils.Lib.Sort.Comparison {
+  import opened Datatypes
+
+  datatype Cmp = Lt | Eq | Gt {
+    function method Flip(): Cmp {
+      match this
+        case Lt => Gt
+        case Eq => Eq
+        case Gt => Lt
+    }
+
+    const Le? := this != Gt
+    const Ge? := this != Lt
+
+    static function method ComputeTransitivity(c0: Cmp, c1: Cmp): Option<Cmp> {
+      match (c0, c1)
+        case (Lt, Lt) => Some(Lt)
+        case (Lt, Eq) => Some(Lt)
+        case (Lt, Gt) => None
+        case (Eq, Lt) => Some(Lt)
+        case (Eq, Eq) => Some(Eq)
+        case (Eq, Gt) => Some(Gt)
+        case (Gt, Lt) => None
+        case (Gt, Eq) => Some(Gt)
+        case (Gt, Gt) => Some(Gt)
+    }
+  }
+
+  datatype Comparison<!T> = Comparison(cmp: (T, T) -> Cmp) {
+    function method Compare(t0: T, t1: T): Cmp {
+      cmp(t0, t1)
+    }
+
+    predicate Complete??(t0: T, t1: T) {
+      cmp(t0, t1) == cmp(t1, t0).Flip()
+    }
+
+    predicate Antisymmetric??(t0: T, t1: T) {
+      cmp(t0, t1) == Eq ==> t0 == t1
+    }
+
+    predicate Transitive??(t0: T, t1: T, t2: T) {
+      cmp(t0, t1).Le? && cmp(t1, t2).Le? ==> cmp(t0, t2).Le?
+    }
+
+    predicate Reflexive??(t0: T) {
+      cmp(t0, t0) == Eq
+    }
+
+    lemma AlwaysReflexive(t0: T)
+      requires Complete??(t0, t0)
+      ensures Reflexive??(t0)
+    {}
+
+    lemma PreciselyTransitive'(t0: T, t1: T, t2: T)
+      requires Complete??(t0, t1) && Complete??(t0, t2) && Complete??(t1, t2)
+      requires Antisymmetric??(t0, t1) && Antisymmetric??(t0, t2) && Antisymmetric??(t1, t2)
+      requires Transitive??(t0, t1, t2) && Transitive??(t1, t2, t0)
+      requires cmp(t0, t1).Le? && cmp(t1, t2).Le?
+      ensures Cmp.ComputeTransitivity(cmp(t0, t1), cmp(t1, t2)) == Some(cmp(t0, t2))
+    {}
+
+    lemma PreciselyTransitive(t0: T, t1: T, t2: T)
+      requires Reflexive??(t0) && Reflexive??(t1) && Reflexive??(t2)
+      requires Complete??(t0, t1) && Complete??(t0, t2) && Complete??(t1, t2)
+      requires Antisymmetric??(t0, t1) && Antisymmetric??(t0, t2) && Antisymmetric??(t1, t2)
+      requires Transitive??(t0, t1, t2) && Transitive??(t1, t2, t0)
+      requires Transitive??(t2, t1, t0) && Transitive??(t1, t0, t2)
+      ensures match Cmp.ComputeTransitivity(cmp(t0, t1), cmp(t1, t2))
+        case Some(c12) => c12 == cmp(t0, t2)
+        case None => true
+    {
+      match (cmp(t0, t1), cmp(t1, t2))
+        case (Lt, Lt) | (Lt, Eq) | (Eq, Lt) | (Eq, Eq) =>
+          PreciselyTransitive'(t0, t1, t2);
+        case (Eq, Gt) | (Gt, Eq) | (Gt, Gt) =>
+          PreciselyTransitive'(t2, t1, t0);
+        case (Lt, Gt) | (Gt, Lt) =>
+    }
+
+    predicate Complete?(ts: set<T>) {
+      forall t0, t1 | t0 in ts && t1 in ts :: Complete??(t0, t1)
+    }
+
+    predicate Antisymmetric?(ts: set<T>) {
+      forall t0, t1 | t0 in ts && t1 in ts :: Antisymmetric??(t0, t1)
+    }
+
+    predicate Transitive?(ts: set<T>) {
+      forall t0, t1, t2 | t0 in ts && t1 in ts && t2 in ts :: Transitive??(t0, t1, t2)
+    }
+
+    predicate Valid?(ts: set<T>) {
+      Complete?(ts) && /* Antisymmetric?(ts) && */ Transitive?(ts)
+    }
+
+    predicate Total?(ts: set<T>) {
+      Complete?(ts) && Antisymmetric?(ts) && Transitive?(ts)
+    }
+
+    predicate Sorted(sq: seq<T>) {
+      forall i, j | 0 <= i < j < |sq| :: cmp(sq[i], sq[j]).Le?
+    }
+
+    lemma SortedConcat(sq0: seq<T>, sq1: seq<T>)
+      requires Sorted(sq0)
+      requires Sorted(sq1)
+      requires forall i, j | 0 <= i < |sq0| && 0 <= j < |sq1| :: cmp(sq0[i], sq1[j]).Le?
+      ensures Sorted(sq0 + sq1)
+    {}
+
+    // lemma SortedUnique(sq0: seq<T>, sq1: seq<T>)
+    //   requires Sorted(sq0)
+    //   requires Sorted(sq1)
+    //   requires multiset(sq0) == multiset(sq1)
+    //   requires Antisymmetric?(set x <- sq0)
+    //   ensures sq0 == sq1
+    // {
+    //   calc { set x <- sq0; set x <- multiset(sq0); set x <- multiset(sq1); set x <- sq1; }
+    // }
+
+    predicate {:opaque} Striped(sq: seq<T>, pivot: T, lo: int, left: int, mid: int, right: int, hi: int)
+      requires 0 <= lo <= left <= mid <= right <= hi <= |sq|
+    {
+      && (forall i | lo    <= i < left :: cmp(sq[i], pivot).Lt?)
+      && (forall i | left  <= i < mid  :: cmp(sq[i], pivot).Eq?)
+      && (forall i | right <= i < hi   :: cmp(sq[i], pivot).Gt?)
+    }
+  }
+}
+
+module Utils.Lib.Sort.DerivedComparison {
+  import C = Comparison
+  import Set
+
+  datatype DerivedComparison<!T, !T'> = DerivedComparison(cmp: C.Comparison<T'>, fn: T -> T') {
+    const Comparison := C.Comparison((t0, t1) => cmp.Compare(fn(t0), fn(t1)));
+
+    lemma Valid(ts: set<T>)
+      requires cmp.Valid?(Set.Map(ts, fn))
+      ensures Comparison.Valid?(ts)
+    {
+      forall s0, s1 | s0 in ts && s1 in ts ensures Comparison.Complete??(s0, s1) {
+        assert cmp.Complete??(fn(s0), fn(s1));
+      }
+      forall s0, s1, s2 | s0 in ts && s1 in ts && s2 in ts ensures Comparison.Transitive??(s0, s1, s2) {
+        assert cmp.Transitive??(fn(s0), fn(s1), fn(s2));
+      }
+    }
+
+    lemma Total(ts: set<T>)
+      requires cmp.Total?(Set.Map(ts, fn))
+      requires forall i, j :: fn(i) == fn(j) ==> i == j
+      ensures Comparison.Total?(ts)
+    {
+      Valid(ts);
+      forall s0, s1 | s0 in ts && s1 in ts ensures Comparison.Antisymmetric??(s0, s1) {
+        calc ==> {
+          Comparison.cmp(s0, s1).Eq?;
+          cmp.cmp(fn(s0), fn(s1)).Eq?;
+          { assert cmp.Antisymmetric??(fn(s0), fn(s1)); }
+          fn(s0) == fn(s1);
+          s0 == s1;
+        }
+      }
+    }
+  }
 }
